rocq-brick-libstdcpp/proof/iostream/itree_prop.v
@@ -1,0 +1,59 @@
+Require Import skylabs.auto.cpp.prelude.proof. (* TODO: reduce dependency *)
+
+Require Import skylabs.auto.hints.kont.
+
+Require Export skylabs.brick.libstdcpp.iostream.itree.
+
+(** A handler for events as a predicate transformer.
+
+    Generally, this will be an <AU> that proves that <evt> is a valid next event.
+ *)
+Record SepHandler {PROP : bi} {evt : Type} : Type :=
+  { do : propset evt -> (evt -> PROP) -> PROP
+    (** This is effectively an <<AU>> that performs the event and then continues *)
+  ; do_frame : forall evtP, ProperFrame (T:=[tele (_ : evt)]) (do evtP)
+  ; do_ne : forall n, Proper ((≡) ==> pointwise_relation _ (dist n) ==> (dist n)) do
+  }.
+#[global] Arguments SepHandler _ _ : clear implicits.
+#[global] Hint Opaque do : sl_opacity.
+
+
+(* TODO: these should be replaced by library definitions *)
+Section interp_itree.
+  Context {PROP : bi}.
+  Context {PROP_LATER : BiLaterContractive PROP}.
+
+  Context {E : Type -> Type}.
+  Context {Evt : Type}.
+  Variable as_evt : forall {T}, E T -> T -> Evt.
+
+  Context (SH : SepHandler PROP Evt).
+
+  #[local]
+  Definition interp_do_body {T} (K : T -> PROP) (rec : itree E T -d> PROP) : itree E T -d> PROP :=
+    funI it =>
+    match it with
+    | Ret v => K v
+    | Tau x => |> rec x
+    | Do act k =>
+        letI* evt := SH.(do) {[ evt | exists r, evt = as_evt act r ]} in
+        ∃ r, [| evt = as_evt act r |] ∗ |> rec (k r)
+    end.
+
+  #[local]
+  Instance interp_do_body_contractive {T} {K : T -> PROP} : Contractive (interp_do_body K).
+  Proof using PROP_LATER.
+    repeat intro.
+    destruct x0; simpl; try eauto.
+    { apply later_contractive. constructor.
+      intros. apply H. done. }
+    { eapply do_ne. done.
+      intro. apply bi.exist_ne; intro. apply bi.sep_ne. done. apply later_contractive.
+      constructor; intros; apply H; done. }
+  Qed.
+
+  Definition interp_itree {T} (it : itree E T) (K : T -> PROP) : PROP :=
+    fixpoint (A:=_ -d> PROP) (interp_do_body K) it.
+
+End interp_itree.
+#[global] Arguments interp_itree {PROP _ E Event} as_evt SH {_} it _%_I : rename.
