rocq-brick-libstdcpp/test/g4g/N6_print_sizeof.v
@@ -32,10 +32,10 @@ Section with_cpp.
   Definition bs_dos_steps_C (s : bs) (s' : propset (Sts._state (App.lts SizeOf))) str
     (ANY_STEPS : AnySteps only_output {[s]} ((fun x => Write x) <$> BS.string_to_bytes str) s') :=
     \cancelx
-      \using{γ} AuthSet.frag γ {[s]}
-      \proving{K : mpredI} ostream.bs_dos (OS:=OS ⊤ γ) str K
-      \through (AuthSet.frag γ s' -∗ K)
-      \end@{mpredI}.
+    \using{γ} AuthSet.frag γ {[s]}
+    \proving{K : mpredI} ostream.bs_dos (OS ⊤ γ) str K
+    \through (AuthSet.frag γ s' -∗ K)
+    \end@{mpredI}.
   Next Obligation.
     simpl.
     intros.
